\documentclass[journal,12pt,twocolumn]{IEEEtran}

\usepackage{tfrupee}
\usepackage{enumitem}
\usepackage{amsmath}
\usepackage{amssymb}


\vspace{3cm}
\title{AI1110 Assignment I (ICSE Class 10 2017)}
\author{Santoshi Gayatri (CS21BTECH11036)}
\date{March 2022}
% make the title area
\begin{document}
\maketitle
\textbf {Question 1:}
If b is the mean proportion between a and c, show that:
$$ \frac{ a^4 + a^2+b^2 + b^4}{b^4 + b^2c^2 + c^2}=\frac{a^2}{c^2}$$\
\textbf{Solution:}
Given that b is mean proporion of a and c. Hence $$a:b:c$$
i.e. $${\frac{a}{b}=\frac{b}{c} }$$
$${\therefore  b^{2}=ac}$$
So we can replace $b^2$ with $ac$ in the LHS\\
Doing that we get,
$$ {LHS = \frac{ a^4 + a^2+b^2 + b^4}{b^4 + b^2c^2 + c^2}}$$\\
$${ = \frac{ a^4 + a^2ac + a^2c^2}{ a^2c^2 + ac^3 + c ^4}}$$\\
$${ = \frac{a^2(a^2 + ac + c^2)}{c^2(a^2 + ac + c^2)}}$$\\
    $${ = \frac{a^2}{c^2}}$$\\[1pt]
\begin{center}
$=RHS$\\
$\therefore LHS=RHS$
\end{center}
Hence proved that, $$ \frac{ a^4 + a^2+b^2 + b^4}{b^4 + b^2c^2 + c^2}=\frac{a^2}{c^2}$$
\end{document}