\documentclass{beamer}
\usetheme{CambridgeUS}

\setbeamertemplate{caption}[numbered]{}

\usepackage{enumitem}
\usepackage{tfrupee}
\usepackage{amsmath}
\usepackage{amssymb}
\usepackage{gensymb}
\usepackage{graphicx}
\usepackage{txfonts}

\def\inputGnumericTable{}

\usepackage[latin1]{inputenc}                                 
\usepackage{color}                                            
\usepackage{array}                                            
\usepackage{longtable}                                        
\usepackage{calc}                                             
\usepackage{multirow}                                         
\usepackage{hhline}                                           
\usepackage{ifthen}
\usepackage{caption} 
\captionsetup[table]{skip=3pt}  
\providecommand{\pr}[1]{\ensuremath{\Pr\left(#1\right)}}
\providecommand{\cbrak}[1]{\ensuremath{\left\{#1\right\}}}
\renewcommand{\thefigure}{\arabic{table}}
\renewcommand{\thetable}{\arabic{table}}                                     
                               
\title{AI1110 \\ Assignment 4}
\author{Santoshi Gayatri Mavuru \\ CS21BTECH11036}
\date{20th May}


\begin{document}
% The title page
\begin{frame}
\titlepage
\end{frame}
	
% The table of contents
\begin{frame}{Outline}
\tableofcontents
\end{frame}
	
\section{Question}
\begin{frame}{CBSE Probability Class 12 Exercise 13 Q12}
Two numbers are selected at random (without replacement) from the first six positive integers. Let X denote the larger of the two numbers obtained. Find E(X).
\end{frame}

\section{Solution}
\begin{frame}{Solution}
Consider first n positive integers.\\
Number of ways to select two random numbers(without replacement) from the first n positive positive integers = 
$ \perm{n}{2} = n(n-1)$. 
\end{frame}

\begin{frame}
Let X represent the larger of the two numbers obtained. Therefore, X can take the values of 2,3,4,5,.... n.
\pr{X=i} where i in ( 2, n)
$ \pr{X=i} = \frac{2(i-1)}{n(n-1)} $
\end{frame}

\begin{frame}
\begin{align}
 E(X) &=\sum_{i = 2}^{i = n}X_iP(X_i) \\
 & = \sum_{i = 2}^{i = n} i * \frac{2(i-1)}{n(n-1)}\\
 & = \frac{2}{n(n-1)} \sum_{i = 1}^{i = n} i^2 + \frac{2}{n(n-1)}\sum_{i = 1}^{i = n} i\\
 & = \frac{2}{n(n-1)} *\frac{n(n+1)(2n+1)}{6} + \frac{2}{n(n-1)} * \frac{n(n+1)}{2}\\
 & = 
 \end{align}
\end{frame}

\begin{frame}
For n = 6, substituting value of 6 in ()\\
$ E(X) = \frac{14}{3} $
\end{frame}
\end{document}